Verify alternate form of composition for graphs

theories/GraphCore/GraphRewriting.v
@@ -7,13 +7,178 @@ From stdpp Require Export pmap gmap.
 
 (* An implementation of double pushout (DPO) rewriting *)
 
+Definition fun_to_map `{Insert A B M, Empty M, Elements A SA}
+  (f : A -> B) (X : SA) : M :=
+  set_to_map (fun a => (a, f a)) X.
 
+Lemma lookup_fun_to_map `{FinMap K M, FinSet K SK, !RelDecision (∈@{SK})} {A}
+  (f : K -> A) (X : SK) k :
+  (fun_to_map f X :> M A) !! k = if decide (k ∈ X) then Some (f k) else None.
+Proof.
+  unfold fun_to_map.
+  case_decide as Hk.
+  - rewrite lookup_set_to_map by done.
+    eauto.
+  - apply eq_None_not_Some.
+    intros (? & Heq).
+    rewrite lookup_set_to_map in Heq by done.
+    now destruct Heq as (_ & ? & [= -> <-]).
+Qed.
+
+
+Lemma lookup_fun_to_map_Some `{FinMap K M, FinSet K SK} {A}
+  (f : K -> A) (X : SK) k a :
+  (fun_to_map f X :> M A) !! k = Some a <->
+  k ∈ X /\ f k = a.
+Proof.
+  unfold fun_to_map.
+  rewrite lookup_set_to_map by done.
+  naive_solver.
+Qed.
+
+Lemma lookup_fun_to_map_None `{FinMap K M, FinSet K SK} {A}
+  (f : K -> A) (X : SK) k :
+  (fun_to_map f X :> M A) !! k = None <->
+  k ∉ X.
+Proof.
+  unfold fun_to_map.
+  rewrite eq_None_not_Some.
+  unfold is_Some.
+  setoid_rewrite lookup_set_to_map; [|done].
+  naive_solver.
+Qed.
+
+Lemma lookup_fun_to_map_Some_1 `{FinMap K M, FinSet K SK} {A}
+  (f : K -> A) (X : SK) k :
+  k ∈ X ->
+  (fun_to_map f X :> M A) !! k = Some (f k).
+Proof.
+  now rewrite lookup_fun_to_map_Some.
+Qed.
+
+Lemma lookup_fun_to_map_None_1 `{FinMap K M, FinSet K SK} {A}
+  (f : K -> A) (X : SK) k :
+  k ∉ X ->
+  (fun_to_map f X :> M A) !! k = None.
+Proof.
+  now rewrite lookup_fun_to_map_None.
+Qed.
+
+
+Lemma lookup_fun_to_map_is_Some `{FinMap K M, FinSet K SK} {A}
+  (f : K -> A) (X : SK) k :
+  is_Some ((fun_to_map f X :> M A) !! k) <-> k ∈ X.
+Proof.
+  unfold is_Some.
+  setoid_rewrite lookup_fun_to_map_Some.
+  naive_solver.
+Qed.
+
+Lemma dom_fun_to_map_gen `{FinMapDom K M SK, FinSet K SK'} {A}
+  (f : K -> A) (X : SK') :
+  dom (fun_to_map f X :> M A) ≡@{SK} set_map id X.
+Proof.
+  intros x.
+  rewrite elem_of_dom.
+  rewrite lookup_fun_to_map_is_Some.
+  set_solver.
+Qed.
+
+Lemma dom_fun_to_map_gen_L `{FinMapDom K M SK, FinSet K SK', !LeibnizEquiv SK} {A}
+  (f : K -> A) (X : SK') :
+  dom (fun_to_map f X :> M A) =@{SK} set_map id X.
+Proof.
+  unfold_leibniz; apply dom_fun_to_map_gen.
+Qed.
+
+Lemma dom_fun_to_map `{FinMapDom K M SK, !Elements K SK, !FinSet K SK} {A}
+  (f : K -> A) (X : SK) :
+  dom (fun_to_map f X :> M A) ≡@{SK} X.
+Proof.
+  now rewrite dom_fun_to_map_gen, set_map_id.
+Qed.
+
+Lemma dom_fun_to_map_L `{FinMapDom K M SK, !Elements K SK,
+  !FinSet K SK, !LeibnizEquiv SK} {A}
+  (f : K -> A) (X : SK) :
+  dom (fun_to_map f X :> M A) =@{SK} X.
+Proof.
+  unfold_leibniz; apply dom_fun_to_map.
+Qed.
+
+Lemma fun_to_map_union `{FinMap K M, FinSet K SK} {A} (f : K -> A)
+  (X Y : SK) :
+  fun_to_map f (X ∪ Y) =@{M A} fun_to_map f X ∪ fun_to_map f Y.
+Proof.
+  apply map_eq.
+  intros k.
+  apply option_eq; intros fk.
+  rewrite lookup_union, union_Some.
+  rewrite 3 lookup_fun_to_map_Some.
+  rewrite elem_of_union.
+  rewrite lookup_fun_to_map_None.
+  pose proof @elem_of_dec_slow.
+  destruct_decide (decide (k ∈ X)); tauto.
+Qed.
+
+Lemma fmap_fun_to_map `{FinMap K M, FinSet K SK} {A B} (f : K -> A) (g : A -> B)
+  (X : SK) :
+  g <$> fun_to_map f X =@{M B} fun_to_map (g ∘ f) X.
+Proof.
+  apply map_eq; intros k.
+  apply option_eq; intros fk.
+  rewrite lookup_fmap, fmap_Some.
+  setoid_rewrite lookup_fun_to_map_Some.
+  naive_solver.
+Qed.
+
+(* Lemma kmap_fun_to_map `{FinMap K1 M1, FinSet K1 SK1, FinMap K2 M2, FinSet K2 SK2}
+  {A} (f : K1 -> A) (g : K1 -> K2) (X : SK1) :
+  kmap g (fun_to_map f X :> M1 A) =@{M2 A}
+    set_to_map (fun a => (g a, f a)) X. *)
+Lemma fun_to_map_singleton
+  `{FinMap K M, FinSet K SK} {A} (f : K -> A)
+  (k : K) :
+  fun_to_map f ({[k]}:>SK) =@{M A} {[k := f k]}.
+Proof.
+  unfold fun_to_map, set_to_map.
+  rewrite elements_singleton.
+  done.
+Qed.
+
+Lemma fun_to_map_difference `{FinMap K M, FinSet K SK} {A} (f : K -> A)
+  (X Y : SK) :
+  fun_to_map f (X ∖ Y) =@{M A} fun_to_map f X ∖ fun_to_map f Y.
+Proof.
+  apply map_eq.
+  intros k.
+  apply option_eq; intros fk.
+  rewrite lookup_difference_Some.
+  rewrite 2 lookup_fun_to_map_Some, lookup_fun_to_map_None.
+  rewrite elem_of_difference.
+  tauto.
+Qed.
+
+Lemma fun_to_map_disjoint `{FinMap K M, FinSet K SK} {A} (f : K -> A)
+  (X Y : SK) : X ## Y -> fun_to_map f X ##ₘ (fun_to_map f Y :> M A).
+Proof.
+  intros HXY.
+  rewrite map_disjoint_alt.
+  intros k.
+  pose proof @elem_of_dec_slow.
+  rewrite 2 lookup_fun_to_map_None.
+  destruct_decide (decide (k ∈ X)).
+  - right.
+    now intros ?; apply (HXY k).
+  - left.
+    now intros ?; apply (HXY k).
+Qed.
 
 Section DPO.
 
 
   Context {T : Type}.
-    
+
 
   (* Definition new_vertex_between {n m} (l r : positive) (tg : CospanHyperGraph T n m) : CospanHyperGraph T n m. *)
 
@@ -32,7 +197,7 @@ Section DPO.
   Fixpoint propogate_subst {n} (ps : vec (positive * positive) n) : vec (positive * positive) n :=
   match n, ps with
   | 0, _ => [#]
-  | (S k), _ => 
+  | (S k), _ =>
     let (p, p') := Vector.hd ps in
     let ps' := Vector.tl ps in
       (p, p') ::: propogate_subst (vmap (relabel_delt ({[p := p']})) ps')
@@ -45,15 +210,107 @@ Section DPO.
     | (a, b) ::: ps' => subst_by_vec ps' ({[a := b]} p)
     end.
 
-  Reserved Notation "tgl ; tgr" (at level 50).
+  (* Reserved Notation "tgl ; tgr" (at level 50). *)
   Definition compose_safe {n m o} (tgl : CospanHyperGraph T n m) (tgr : CospanHyperGraph T m o) : CospanHyperGraph T n o :=
-    let connected_substs := 
-        propogate_subst (vzip (vmap (bcons false) tgl.(outputs)) (vmap (bcons true) tgr.(inputs))) in 
+    let connected_substs :=
+        propogate_subst (vzip (vmap (bcons false) tgl.(outputs)) (vmap (bcons true) tgr.(inputs))) in
      relabel_graph (subst_by_vec connected_substs) ((vmap (bcons false) tgl.(inputs)) -> tgl.(hedges) ⊎ tgr.(hedges) <- (vmap (bcons true) tgr.(outputs))).
 
   Definition compose {n m o} (tgl : CospanHyperGraph T n m) (tgr : CospanHyperGraph T m o) : CospanHyperGraph T n o :=
     let connected_substs := propogate_subst (vzip (tgl.(outputs)) (tgr.(inputs))) in
-    relabel_graph (subst_by_vec connected_substs) 
+    relabel_graph (subst_by_vec connected_substs)
       (tgl.(inputs) -> tgl.(hedges) ∪ tgr.(hedges) <- tgr.(outputs)).
 
+Lemma compose_safe_to_compose {n m o}
+  (tgl : CospanHyperGraph T n m) (tgr : CospanHyperGraph T m o) :
+  compose_safe tgl tgr = compose
+    (reindex_graph (bcons false) (relabel_graph (bcons false) tgl))
+    (reindex_graph (bcons true) (relabel_graph (bcons true) tgr)).
+Proof.
+  reflexivity.
+Qed.
+
+(* Definition graph_disj {n m n' m'} (tg : CospanHyperGraph T n m)
+  (tg' : CospanHyperGraph T n' m') : Prop :=
+   *)
+
+Lemma relabel_hg_union f (hg hg' : HyperGraph T) :
+  relabel_hg f (hg ∪ hg') =
+  relabel_hg f hg ∪ relabel_hg f hg'.
+Proof.
+  apply hg_ext; cbn.
+  - now rewrite map_fmap_union.
+  - now rewrite set_map_union_L.
+Qed.
+
+(* Lemma propogate_subst_vmap {n} (fl fr : positive -> positive)
+  `{Hfl : !Inj eq eq fl, Hfr : !Inj eq eq fr} 
+  (Hf : forall i j, fl i <> fr j) (v : vec _ n) :
+  v.*1 ## v.*2 ->
+  propogate_subst (vmap (prod_map fl fr) v) =
+  vmap (prod_map fl fr) (propogate_subst v).
+Proof.
+  revert v; induction n as [|n IHn]; [refine (vec_0_inv _ _);done|
+    refine (vec_S_inv _ _)].
+  intros (p, q) v.
+  cbn.
+  intros Hdisj.
+  f_equal.
+  rewrite <- IHn.
+  f_equal.
+  apply vec_eq; intros i.
+  rewrite 2 Vector.map_map, 2 vlookup_map.
+  destruct (v !!! i) as (pi, qi).
+  cbn.
+  rewrite fn_lookup_singleton_case.
+  rewrite fn_lookup_singleton_ne by eauto.
+
+  rewrite fnlookup
+  f_equiv.
+
+
+Lemma compose_relabel_graph {n m o} fl fr
+  `{Hfl : !Inj eq eq fl, Hfr : !Inj eq eq fr}
+  (tgl : CospanHyperGraph T n m) (tgr : CospanHyperGraph T m o) :
+  vertices tgl ## vertices tgr ->
+  compose (relabel_graph fl tgl) (relabel_graph fr tgr) =
+  relabel_graph (
+    Pmap_map (fun_to_map fl (vertices tgl) ∪
+      fun_to_map fr (vertices tgr))) (compose tgl tgr).
+Proof.
+  intros Hdisj.
+  apply cohg_ext.
+  - cbn.
+    rewrite relabel_hg_compose.
+    rewrite 2 relabel_hg_union, 2 relabel_hg_compose.
+    f_equal.
+    + apply relabel_hg_ext_strong.
+      intros i Hi.
+      rewrite vzip_map.
+
+
+
+
+Lemma compose_isomorphic {n m o}
+  (tgl tgl' : CospanHyperGraph T n m) (tgr tgr' : CospanHyperGraph T m o) :
+  isomorphic tgl tgl' -> isomorphic tgr tgr' ->
+  isomorphic (compose tgl tgr) (compose tgl' tgr').
+Proof.
+  intros (fle & flv & Hfle & Hflv & ->)%isomorphic_exists
+    (fre & frv & Hfre & Hfrv & ->)%isomorphic_exists.
+  apply isomorphic_exists.
+  exists (pos_map fle fre), (pos_map flv frv).
+  split; [apply _|].
+  split; [apply _|].
+
+
+Lemma compose_graphs_alt_correct {n m o}
+  (tgl : CospanHyperGraph T n m) (tgr : CospanHyperGraph T m o) :
+  isomorphic (compose_graphs_alt tgl tgr)
+    (compose_safe tgl tgr).
+Proof. *)
+
+
+
 End DPO.
+
