theories/GraphCore/TensorGraphFacts.v
@@ -11,6 +11,90 @@ Require TECospan.
 
 Open Scope nat_scope.
 
+Definition abstracts_indices {A} (abs : list (Idx * list A * list A)) : Pset :=
+  list_to_set ((fst ∘ fst) <$> abs).
+
+Lemma abstracts_indices_ntl2tl ntl :
+  abstracts_indices (ntl2tl ntl).(tl_abstracts) =
+  abstracts_indices ntl.(ntl_abstracts).
+Proof.
+  destruct ntl as [isums abs].
+  cbn.
+  rewrite <- list_fmap_compose.
+  f_equal.
+  apply list_fmap_ext; now intros _ [[]] _.
+Qed.
+
+Lemma abstracts_indices_relabel_abs `(f : A -> B) abs :
+  abstracts_indices (relabel_abs f <$> abs) = abstracts_indices abs.
+Proof.
+  unfold abstracts_indices.
+  rewrite <- list_fmap_compose.
+  f_equal.
+  now apply list_fmap_ext; intros _ [[]] _.
+Qed.
+
+Lemma abstracts_indices_ntl_aeq ntl ntl' :
+  ntl =ntl= ntl' ->
+  abstracts_indices ntl.(ntl_abstracts) =
+  abstracts_indices ntl'.(ntl_abstracts).
+Proof.
+  intros (f & _ & _ & Habs & Hdelt).
+  unfold abstracts_indices.
+  rewrite <- Habs.
+  symmetry.
+  apply abstracts_indices_relabel_abs.
+Qed.
+
+Lemma tl_total_semantics_aux_absidxs_ext
+  `{SR : SemiRing R rO rI radd rmul req, SA : Summable A, AEQ : EqDecision A}
+  mabs mabs' ml mr sums abs delt :
+  (forall i, i ∈ abstracts_indices abs -> mabs !! i = mabs' !! i) ->
+  req (tl_total_semantics_aux (SR:=SR) mabs ml mr sums abs delt)
+    (tl_total_semantics_aux mabs' ml mr sums abs delt).
+Proof.
+  intros Habs.
+  revert mr;
+  induction sums; intros mr;
+  [|cbn; apply sum_of_ext; intros ?; apply IHsums].
+  apply tl_total_semantics_aux_ext_base; apply Forall_Forall2_diag;
+  rewrite Forall_forall.
+  - intros [[f low] up] Hflu.
+    split; [|split; apply Forall_Forall2_diag;
+      rewrite Forall_forall; intros; reflexivity].
+    cbn.
+    apply Habs.
+    set_unfold.
+    now exists (f, low, up).
+  - easy.
+Qed.
+
+Lemma ntl_total_semantics_absidxs_ext
+  `{SR : SemiRing R rO rI radd rmul req, SA : Summable A, AEQ : EqDecision A}
+  mabs mabs' ml ntl :
+  (forall i, i ∈ abstracts_indices ntl.(ntl_abstracts) -> mabs !! i = mabs' !! i) ->
+  req (ntl_total_semantics (SR:=SR) mabs ml ntl)
+    (ntl_total_semantics mabs' ml ntl).
+Proof.
+  intros Habs.
+  apply tl_total_semantics_aux_absidxs_ext.
+  destruct ntl as [isums abs delt].
+  rewrite abstracts_indices_ntl2tl.
+  apply Habs.
+Qed.
+
+
+Lemma ntl_total_semantics_relabel_free
+  `{SR : SemiRing R rO rI radd rmul req, SA : Summable A, AEQ : EqDecision A}
+  f `{Hf : !Inj eq eq f} mabs ml ntl :
+  req (ntl_total_semantics (SR:=SR) mabs (kmap f ml) (relabel_ntl_free f ntl))
+    (ntl_total_semantics mabs ml ntl).
+Proof.
+  unfold ntl_total_semantics.
+  rewrite ntl2tl_relabel_ntl_free.
+  apply (relabel_tl_free_semantics_aux_kmap _).
+Qed.
+
 (* FIXME: Move *)
 Lemma forall_var (P : var -> Prop) :
   (forall v, P v) <-> (forall r, P (bound r)) /\ (forall l, P (free l)).
@@ -18,6 +102,33 @@ Proof.
   split; [auto|].
   now intros (?&?) [].
 Qed.
+Lemma map_to_list_disj_union `{FinMap K M} {A} (m1 m2 : M A) :
+  m1 ##ₘ m2 ->
+  map_to_list (m1 ∪ m2) ≡ₚ map_to_list m1 ++ map_to_list m2.
+Proof.
+  intros Hdisj.
+  pose proof Hdisj as Hdisj'.
+  rewrite map_disjoint_alt in Hdisj'.
+  apply NoDup_Permutation.
+  - apply NoDup_map_to_list.
+  - apply NoDup_app; split_and!; try apply NoDup_map_to_list.
+    intros (k, a) Hka%elem_of_map_to_list Hka'%elem_of_map_to_list.
+    destruct (Hdisj' k); congruence.
+  - intros (k, a).
+    rewrite elem_of_app, 3 elem_of_map_to_list.
+    rewrite lookup_union_Some by done.
+    done.
+Qed.
+Lemma map_to_list_kmap `{FinMap K1 M1, FinMap K2 M2} (f : K1 -> K2)
+  `{Hf : !Inj eq eq f} {A} (m : M1 A) :
+  map_to_list (kmap f m :> M2 A) ≡ₚ prod_map f id <$> map_to_list m.
+Proof.
+  unfold kmap.
+  apply map_to_list_to_map.
+  rewrite fsts_prod_map, (NoDup_fmap _).
+  apply NoDup_fst_map_to_list.
+Qed.
+
 
 
 
@@ -250,7 +361,7 @@ Proof.
   intros v w Hv Hw.
   (* rewrite <- reindex_relabel_graph. *)
   unfold graph_semantics, namedtensorlist_to_tensor.
-  cbn -[ntl_total_semantics make_ml graph_mabs].
+  cbn -[ntl_total_semantics make_vecs_map graph_mabs].
   symmetry.
   erewrite ntl_aeq_correct;
   [|apply graph_namedtensorlist_semantics_WF|].
@@ -300,6 +411,15 @@ Lemma tg_list_to_deltas_fmap b f ioputs :
   relabel_delt (relabel_bounds f) <$> tg_list_to_deltas b ioputs.
 Proof.
   unfold tg_list_to_deltas.
+  rewrite fmap_imap, imap_fmap.
+  reflexivity.
+Qed.
+
+Lemma tg_list_to_deltas_offset_fmap off b f ioputs :
+  tg_list_to_deltas_offset off b (f <$> ioputs) =
+  relabel_delt (relabel_bounds f) <$> tg_list_to_deltas_offset off b ioputs.
+Proof.
+  unfold tg_list_to_deltas_offset.
   rewrite fmap_imap, imap_fmap.
   reflexivity.
 Qed.
@@ -369,11 +489,6 @@ Qed.
 
 Import TECospan.
 
-Definition graph_contl_semantics {n m} (tg : TensorGraph n m) :
-  CospanNamedTensorList n m :=
-  mk_contl (graph_namedtensorlist_semantics tg)
-    (vmap (bcons false ∘ Pos.of_succ_nat) $ vseq 0 n)
-    (vmap (bcons true ∘ Pos.of_succ_nat) $ vseq 0 m).
 
 
 
@@ -445,8 +560,9 @@ Proof.
   apply ntl_delta_eq_idemp with v; easy.
 Qed.
 
-Lemma tg_abstracts_relabel_abs (f : positive -> positive) (hg : HyperGraph T) :
-  tg_abstracts (relabel_abs f <$> hg.(hyperedges)) =
+Lemma tg_abstracts_relabel_abs (f : positive -> positive)
+  (hg : Pmap (T * _ * _)) :
+  tg_abstracts (relabel_abs f <$> hg) =
   relabel_abs (relabel_bounds f) <$> tg_abstracts hg.
 Proof.
   unfold tg_abstracts.
@@ -707,28 +823,307 @@ Proof.
       lia.
 Qed.
 
+Lemma contl_eq_of_ntl_eq' {n m}
+  (contl : CospanNamedTensorList n m) (contl' : CospanNamedTensorList n m) :
+  contl.(contl_inputs) = contl'.(contl_inputs) ->
+  contl.(contl_outputs) = contl'.(contl_outputs) ->
+  ntl_eq (contl_boundary contl) contl contl' ->
+  contl_eq contl contl'.
+Proof.
+  destruct contl as [ntl ins outs], contl' as [ntl' ins' outs'].
+  cbn.
+  intros <- <-.
+  apply contl_eq_of_ntl_eq.
+Qed.
+
+
+Lemma vertices_hg_union (hg hg' : HyperGraph T) :
+  (hg :> Pmap _) ##ₘ (hg' :> Pmap _) ->
+  vertices_hg (hg ∪ hg') =
+  vertices_hg hg ∪ vertices_hg hg'.
+Proof.
+  intros Hdisj.
+  apply set_eq.
+  intros x.
+  rewrite elem_of_union, 3 elem_of_vertices_hg.
+  change (hypervertices (_ ∪ _)) with (hypervertices hg ∪ hypervertices hg').
+  rewrite elem_of_union.
+  setoid_rewrite lookup_union_Some; [|done].
+  naive_solver.
+Qed.
+
+Lemma tg_abstracts_union (hg hg' : Pmap (T * _ * _)) :
+  (hg :> Pmap _) ##ₘ (hg' :> Pmap _) ->
+  tg_abstracts (hg ∪ hg') ≡ₚ
+  tg_abstracts hg ++ tg_abstracts hg'.
+Proof.
+  intros Hdisj.
+  unfold tg_abstracts.
+  cbn.
+  rewrite map_to_list_disj_union by done.
+  now rewrite fmap_app.
+Qed.
+
+Lemma vertices_swapped_stack_graphs_aux {n m n' m'}
+  (tg : TensorGraph n m) (tg' : TensorGraph n' m') :
+  tg.(hedges).(hyperedges) ##ₘ tg'.(hedges).(hyperedges) ->
+  vertices (swapped_stack_graphs_aux tg tg') =
+  vertices tg ∪ vertices tg'.
+Proof.
+  intros Hdisj.
+  unfold vertices; cbn.
+  rewrite vertices_hg_union by done.
+  rewrite 2 vec_to_list_app, 5 list_to_set_app_L.
+  apply set_eq; intros x.
+  rewrite 10 elem_of_union. tauto.
+Qed.
+
+Lemma vertices_swapped_stack_graphs {n m n' m'}
+  (tg : TensorGraph n m) (tg' : TensorGraph n' m') :
+  vertices (swapped_stack_graphs tg tg') =
+  set_map (bcons false) (vertices tg) ∪
+  set_map (bcons true) (vertices tg').
+Proof.
+  unfold swapped_stack_graphs.
+  rewrite vertices_swapped_stack_graphs_aux.
+  - now rewrite 2 vertices_relabel_graph, 2 (vertices_reindex_graph _).
+  - cbn.
+    rewrite map_disjoint_fmap.
+    rewrite map_disjoint_alt.
+    intros [].
+    + left.
+      apply (lookup_kmap_None _); lia.
+    + right.
+      apply (lookup_kmap_None _); lia.
+    + left.
+      apply (lookup_kmap_None _); lia.
+Qed.
+
+(* Lemma graph_contl_semantics_swapped_stack {n m n' m'}
+  (tg : TensorGraph n m) (tg' : TensorGraph n' m') :
+  contl_eq (graph_contl_semantics (swapped_stack_graphs tg tg'))
+  (swapped_stack_contl
+    ((graph_contl_semantics tg))
+    ((graph_contl_semantics tg'))).
+Proof.
+  etransitivity. 1:{
+    apply (fun H => @contl_eq_relabel_free
+      (pos_elim (λ i, if decide (i < n') then i~0~1
+        else (pos_sub_N i (N.of_nat n'))~0~0)
+        (λ i, if decide (i < m) then i~1~0
+          else (pos_sub_N i (N.of_nat m))~1~1) ) H).
+    admit.
+  }
+  apply contl_eq_of_ntl_eq', ntl_eq_of_ntl_aeq, ntl_aeq_of_perm.
+  - cbn.
+    apply vec_to_list_inj2.
+    rewrite 3 Vector.map_map, vec_to_list_app, 3 vec_to_list_map,
+      3 vec_to_list_seq, seq_app, fmap_app, (Nat.add_comm 0),
+        <- (fmap_add_seq), <- list_fmap_compose.
+    f_equal.
+    + unfold compose.
+      cbn.
+      apply list_fmap_ext; intros _ ? Hx%elem_of_list_lookup_2%elem_of_seq;
+      apply decide_True; lia.
+    + unfold compose.
+      cbn.
+      apply list_fmap_ext; intros _ ? Hx%elem_of_list_lookup_2%elem_of_seq.
+      rewrite decide_False by lia.
+      lia.
+  - cbn.
+    apply vec_to_list_inj2.
+    rewrite 3 Vector.map_map, vec_to_list_app, 3 vec_to_list_map,
+      3 vec_to_list_seq, seq_app, fmap_app, (Nat.add_comm 0),
+        <- (fmap_add_seq), <- list_fmap_compose.
+    f_equal.
+    + unfold compose.
+      cbn.
+      apply list_fmap_ext; intros _ ? Hx%elem_of_list_lookup_2%elem_of_seq;
+      apply decide_True; lia.
+    + unfold compose.
+      cbn.
+      apply list_fmap_ext; intros _ ? Hx%elem_of_list_lookup_2%elem_of_seq.
+      rewrite decide_False by lia.
+      lia.
+  - cbn.
+    rewrite vertices_swapped_stack_graphs.
+      rewrite elements_disj_union by set_solver.
+      now rewrite <- 2 (fmap_elements _).
+  - cbn.
+
+    rewrite tg_abstracts_union by
+      now apply map_disjoint_dom;
+      rewrite 2 dom_fmap, 2 dom_kmap_L';
+      set_solver.
+    rewrite 2 tg_abstracts_relabel_abs.
+
+    apply vec_to_list_inj2.
+    rewrite 2 Vector.map_map, vec_to_list_app, 3 vec_to_list_map,
+      3 vec_to_list_seq, seq_app, fmap_app, (Nat.add_comm 0),
+        <- (fmap_add_seq), <- list_fmap_compose.
+    f_equal.
+    unfold compose.
+    cbn.
+    apply list_fmap_ext; lia.
+  - cbn.
+    apply vec_to_list_inj2.
+    rewrite 2 Vector.map_map, vec_to_list_app, 3 vec_to_list_map,
+      3 vec_to_list_seq, seq_app, fmap_app, (Nat.add_comm 0),
+        <- (fmap_add_seq), <- list_fmap_compose.
+    f_equal.
+    unfold compose.
+    cbn.
+    apply list_fmap_ext; lia.
+  - cbn.
+    unfold vertices; cbn. *)
+
+(* Lemma graph_contl_semantics_swapped_stack {n m n' m'}
+  (tg : TensorGraph n m) (tg' : TensorGraph n' m') :
+  contl_eq (graph_contl_semantics (swapped_stack_graphs_aux tg tg'))
+  (swapped_stack_contl_aux
+    (relabel_contl_free (pos_map (λ p, pos_add_N p (N.of_nat n')) id)
+      (graph_contl_semantics tg))
+    (relabel_contl_free (pos_map id (λ p, pos_add_N p (N.of_nat m)))
+      (graph_contl_semantics tg'))).
+Proof.
+  apply contl_eq_of_ntl_eq', ntl_eq_of_ntl_aeq, ntl_aeq_of_perm.
+  - cbn.
+    apply vec_to_list_inj2.
+    rewrite 2 Vector.map_map, vec_to_list_app, 3 vec_to_list_map,
+      3 vec_to_list_seq, seq_app, fmap_app, (Nat.add_comm 0),
+        <- (fmap_add_seq), <- list_fmap_compose.
+    f_equal.
+    unfold compose.
+    cbn.
+    apply list_fmap_ext; lia.
+  - cbn.
+    apply vec_to_list_inj2.
+    rewrite 2 Vector.map_map, vec_to_list_app, 3 vec_to_list_map,
+      3 vec_to_list_seq, seq_app, fmap_app, (Nat.add_comm 0),
+        <- (fmap_add_seq), <- list_fmap_compose.
+    f_equal.
+    unfold compose.
+    cbn.
+    apply list_fmap_ext; lia.
+  - cbn.
+    unfold vertices; cbn. *)
+
+Lemma tg_abstracts_kmap f `{Hf : !Inj eq eq f} (hg : Pmap (T * _ * _)) :
+  tg_abstracts (kmap f hg) ≡ₚ
+  prod_map (prod_map f id) id <$> tg_abstracts hg.
+Proof.
+  unfold tg_abstracts.
+  rewrite (map_to_list_kmap _).
+  rewrite <- 2 list_fmap_compose.
+  done.
+Qed.
+
+Lemma relabel_ntl_free_ntl_times f ntl ntl' :
+  relabel_ntl_free f (ntl_times ntl ntl') =
+  ntl_times (relabel_ntl_free f ntl) (relabel_ntl_free f ntl').
+Proof.
+  apply ntl_ext; cbn.
+  - done.
+  - rewrite fmap_app, <- 4 list_fmap_compose.
+    f_equal;
+    now apply list_fmap_ext; intros _ flu _; cbn;
+    rewrite 2 relabel_abs_compose;
+    apply relabel_abs_ext; intros [].
+  - rewrite fmap_app, <- 4 list_fmap_compose.
+    f_equal;
+    now apply list_fmap_ext; intros _ lu _; cbn;
+    rewrite 2 relabel_delt_compose;
+    apply relabel_delt_ext; intros [].
+Qed.
+
+Lemma tg_list_to_deltas_app out idxs idxs' :
+  tg_list_to_deltas out (idxs ++ idxs') =
+  tg_list_to_deltas out idxs ++
+  tg_list_to_deltas_offset (length idxs) out idxs'.
+Proof.
+  refine (imap_app _ _ _).
+Qed.
+
+Lemma graph_namedtensorlist_semantics_swapped_stack_graphs {n m n' m'}
+  (cohg : TensorGraph n m) (cohg' : TensorGraph n' m') :
+  graph_namedtensorlist_semantics (swapped_stack_graphs cohg cohg') =ntl=
+  ntl_times
+    (ntl_relabel_absidx (bcons false)
+      (graph_namedtensorlist_semantics_offset n' 0 cohg))
+    (ntl_relabel_absidx (bcons true)
+      (graph_namedtensorlist_semantics_offset 0 m cohg')).
+Proof.
+  apply ntl_aeq_of_perm.
+  - cbn.
+    rewrite vertices_swapped_stack_graphs.
+    rewrite elements_disj_union by set_solver.
+    now rewrite <- 2 (fmap_elements _).
+  - cbn.
+    rewrite tg_abstracts_union by
+      now apply map_disjoint_dom;
+      rewrite 2 dom_fmap, 2 dom_kmap_L';
+      set_solver.
+    rewrite 2 tg_abstracts_relabel_abs.
+    rewrite 2 (tg_abstracts_kmap _).
+    done.
+  - cbn -[tg_list_to_deltas].
+    rewrite 2 vec_to_list_app, 2 tg_list_to_deltas_app, 2 length_vec_to_list.
+    rewrite 4 vec_to_list_map.
+    rewrite 2 tg_list_to_deltas_fmap, 2 tg_list_to_deltas_offset_fmap.
+    rewrite 2 fmap_app.
+    solve_Permutation.
+Qed.
 
 
 
+
+
+
+
+Context `{!WFSummable A}.
+
+
+Lemma graph_mabs_relabel_abs f (hg : Pmap (HyperEdge T)) :
+  graph_mabs (relabel_abs f <$> hg) =
+  graph_mabs hg.
+Proof.
+  unfold graph_mabs; cbn.
+  rewrite <- map_fmap_compose.
+  apply map_fmap_ext; intros _ [[]] _;
+  done.
+Qed.
+
+Lemma graph_mabs_relabel_graph f {n m} (tg : TensorGraph n m) :
+  graph_mabs (relabel_graph f tg).(hedges) = graph_mabs tg.(hedges).
+Proof.
+  apply graph_mabs_relabel_abs.
+Qed.
+
+
+Lemma graph_mabs_add_top_loop {n m} (tg : TensorGraph (S n) (S m)) :
+  graph_mabs (add_top_loop tg).(hedges) = graph_mabs tg.(hedges).
+Proof.
+  apply (@graph_mabs_relabel_graph _ (S n) (S m)).
+Qed.
 
 
 Lemma graph_semantics_add_top_loop {n m} (tg : TensorGraph (S n) (S m)) :
   graph_semantics (add_top_loop tg) ≡
   join_stack_1_tl_tr (graph_semantics (SR:=SR) tg).
 Proof.
-  intros v w Hv Hw.
-  cbn -[graph_semantics].
-  unfold graph_semantics, namedtensorlist_to_tensor.
-  rewrite ntl_total_semantics_alt by now apply graph_namedtensorlist_semantics_WF.
-  setoid_rewrite ntl_total_semantics_alt; last
-    now apply graph_namedtensorlist_semantics_WF.
-  destruct tg as [hedges ins outs].
-  induction ins as [i ins] using vec_S_inv.
-  induction outs as [o outs] using vec_S_inv.
-
-
-  cbn -[abstracts_semantics_alt deltas_semantics_alt list_to_map vmap vseq].
-Admitted.
+  rewrite 2 graph_semantics_to_contl.
+  rewrite <- contl_semantics_add_top_loop_gen.
+  - rewrite graph_mabs_add_top_loop.
+    apply contl_eq_correct, graph_contl_semantics_add_top_loop.
+    apply graph_contl_semantics_WT.
+  - apply graph_contl_semantics_WT.
+  - cbn.
+    rewrite vec_to_list_map, vec_to_list_seq.
+    rewrite elem_of_list_fmap.
+    intros (? & ? & _).
+    cbn in *.
+    lia.
+Qed.
 
 Lemma graph_semantics_add_top_loops {n m o} (tg : TensorGraph (n + m) (n + o)) :
   graph_semantics (add_top_loops tg) ≡
@@ -739,6 +1134,253 @@ Proof.
   rewrite IHn.
   apply join_stack_tl_tr_mor.
   apply graph_semantics_add_top_loop.
+Qed.
+
+
+Lemma abstracts_indices_relabel_absidx f ntl :
+  abstracts_indices (ntl_relabel_absidx f ntl).(ntl_abstracts) =
+  set_map f (abstracts_indices ntl.(ntl_abstracts)).
+Proof.
+  unfold abstracts_indices.
+  cbn.
+  rewrite <- list_fmap_compose.
+  unfold compose, prod_map; cbn.
+  rewrite set_map_list_to_set_L.
+  rewrite <- list_fmap_compose.
+  done.
+Qed.
+
+Lemma ntl_relabel_absidx_relabel_free f g ntl :
+  ntl_relabel_absidx f (relabel_ntl_free g ntl) =
+  relabel_ntl_free g (ntl_relabel_absidx f ntl).
+Proof.
+  unfold ntl_relabel_absidx, relabel_ntl_free.
+  cbn.
+  f_equal.
+  rewrite <- 2 list_fmap_compose.
+  apply list_fmap_ext; now intros _ [[]] _.
+Qed.
+
+Lemma graph_namedtensorlist_semantics_offset_WF noff moff `(tg : TensorGraph n m) :
+  WF_ntl (graph_namedtensorlist_semantics_offset noff moff tg).
+Proof.
+  rewrite graph_namedtensorlist_semantics_offset_correct.
+  apply relabel_ntl_free_WF, graph_namedtensorlist_semantics_WF.
+Qed.
+
+Lemma graph_mabs_union (hg hg' : Pmap (HyperEdge T)) :
+  graph_mabs (hg ∪ hg') =
+  graph_mabs hg ∪ graph_mabs hg'.
+Proof.
+  unfold graph_mabs.
+  rewrite map_fmap_union.
+  done.
+Qed.
+
+Lemma graph_mabs_kmap f (hg : Pmap (HyperEdge T)) :
+  graph_mabs (kmap f hg) = kmap f (graph_mabs hg).
+Proof.
+  symmetry;
+  apply kmap_fmap'.
+Qed.
+Lemma ntl_free_varset_relabel_absidx f ntl :
+  ntl_free_varset (ntl_relabel_absidx f ntl) = ntl_free_varset ntl.
+Proof.
+  unfold ntl_free_varset.
+  cbn.
+  f_equal.
+  unfold abstracts_free_vars.
+  rewrite list_fmap_bind.
+  unfold compose.
+  f_equal.
+  apply list_bind_ext; [now intros [[]]|done].
+Qed.
+
+
+
+(* FIXME: Move *)
+#[global] Arguments graph_semantics {_ _ _}
+  {_ _ _ _ _ _} {_ _ _} {_ _} _ _ _ / : assert.
+
+Lemma graph_semantics_swapped_stack_graphs {n m n' m'}
+  (cohg : TensorGraph n m) (cohg' : TensorGraph n' m') :
+  graph_semantics (SR:=SR) (swapped_stack_graphs cohg cohg') ≡
+  swapped_stack_tensor (graph_semantics cohg) (graph_semantics cohg').
+Proof.
+  intros v w Hv Hw.
+
+  induction v as [vl vr] using vec_add_inv.
+  induction w as [wl wr] using vec_add_inv.
+  rewrite 3 graph_semantics_to_contl.
+  cbn -[ntl_total_semantics ntl_times graph_mabs].
+  rewrite 2 vsplitl_app, 2 vsplitr_app.
+  unfold graph_contl_semantics, contl_semantics;
+  cbn -[ntl_total_semantics ntl_times graph_mabs make_vecs_map].
+  erewrite ntl_aeq_correct by first [apply graph_namedtensorlist_semantics_WF|
+    apply graph_namedtensorlist_semantics_swapped_stack_graphs].
+  rewrite ntl_total_semantics_ntl_times by now apply ntl_relabel_absidx_WF,
+    graph_namedtensorlist_semantics_offset_WF.
+  f_equiv.
+  - rewrite graph_namedtensorlist_semantics_offset_correct.
+    symmetry.
+    rewrite <- (relabel_ntl_free_semantics_kmap _ _ (pos_map (pos_nat_add n') (pos_nat_add 0))).
+    rewrite <- (ntl_total_semantics_kmap_ntl_relabel_absidx _ _ (bcons false)).
+    rewrite graph_mabs_union, 2 graph_mabs_relabel_abs, 2 graph_mabs_kmap.
+
+    etransitivity; [apply ntl_total_semantics_absidxs_ext|
+      apply ntl_total_semantics_free_varset_ext].
+    + rewrite abstracts_indices_relabel_absidx.
+      cbn -[abstracts_indices].
+      rewrite abstracts_indices_relabel_abs.
+      intros _ (i & -> & Hi)%elem_of_map.
+      rewrite lookup_union.
+      rewrite (lookup_kmap_None (bcons true) _ _).2 by lia.
+      now rewrite (right_id None _).
+    + rewrite ntl_free_varset_relabel_absidx, ntl_free_varset_relabel_ntl_free.
+      intros _ (i & -> & Hi)%elem_of_map.
+      rewrite (lookup_kmap _).
+      unfold make_vecs_map.
+      rewrite 4 vzip_map_l, 4 vec_to_list_map.
+      rewrite <- 4 (kmap_list_to_map _).
+      rewrite 2 lookup_union.
+      destruct i as [i|i|].
+      * replace (i~1) with ((bcons true ∘ Pos.of_succ_nat) i) by now cbn; lia.
+        rewrite (lookup_kmap_None (bcons false ∘ _) _ _).2 by now cbn; lia.
+        rewrite (lookup_kmap _).
+        cbn.
+        change (?x~1) with ((bcons true ∘ Pos.of_succ_nat) i).
+        rewrite (lookup_kmap _).
+        rewrite (lookup_kmap_None _ _ _).2 by now cbn; lia.
+        f_equal.
+        rewrite vec_to_list_zip_with, vec_to_list_seq.
+        rewrite <- (length_vec_to_list wl) at 1.
+        rewrite <- imap_to_zip_with_seq.
+        rewrite vec_to_list_zip_with, vec_to_list_seq.
+        rewrite <- (length_vec_to_list (wl +++ wr)) at 1.
+        rewrite <- imap_to_zip_with_seq.
+        setoid_rewrite (lookup_list_to_map_imap id id _ (pos_to_nat_pred i)).
+        rewrite 2option_fmap_id.
+        rewrite vec_to_list_app.
+        symmetry.
+        apply lookup_app_l.
+        rewrite ntl_free_varset_graph in Hi.
+        rewrite elem_of_list_to_set in Hi.
+        rewrite 2 vec_to_list_map, 2 vec_to_list_seq in Hi.
+        set_unfold in Hi.
+        setoid_rewrite elem_of_seq in Hi.
+        cbn in Hi.
+        rewrite length_vec_to_list.
+        firstorder lia.
+      * replace (i~0) with ((bcons false ∘ Pos.of_succ_nat) i) by now cbn; lia.
+        rewrite (lookup_kmap_None (bcons true ∘ _) _ _).2 by now cbn; lia.
+        rewrite (lookup_kmap _).
+        cbn.
+        replace (_~0) with ((bcons false ∘ Pos.of_succ_nat) (n' + i)) by now cbn; lia.
+        rewrite (lookup_kmap _).
+        rewrite (lookup_kmap_None _ _ _).2 by now cbn; lia.
+        f_equal.
+        rewrite vec_to_list_zip_with, vec_to_list_seq.
+        rewrite <- (length_vec_to_list vr) at 1.
+        rewrite <- imap_to_zip_with_seq.
+        rewrite vec_to_list_zip_with, vec_to_list_seq.
+        rewrite <- (length_vec_to_list (vl +++ vr)) at 1.
+        rewrite <- imap_to_zip_with_seq.
+        rewrite (lookup_list_to_map_imap id id _ (pos_to_nat_pred i)).
+        rewrite (lookup_list_to_map_imap id id _ (n' + i)).
+        rewrite 2 option_fmap_id.
+        rewrite vec_to_list_app.
+        symmetry.
+        rewrite lookup_app_r; [f_equal; rewrite length_vec_to_list; lia|].
+        rewrite length_vec_to_list.
+        lia.
+      * rewrite 4(lookup_kmap_None _ _ _).2 by now cbn; lia.
+        done.
+  - rewrite graph_namedtensorlist_semantics_offset_correct.
+    symmetry.
+    rewrite <- (relabel_ntl_free_semantics_kmap _ _ (pos_map (pos_nat_add 0) (pos_nat_add m))).
+    rewrite <- (ntl_total_semantics_kmap_ntl_relabel_absidx _ _ (bcons true)).
+    rewrite graph_mabs_union, 2 graph_mabs_relabel_abs, 2 graph_mabs_kmap.
+
+    etransitivity; [apply ntl_total_semantics_absidxs_ext|
+      apply ntl_total_semantics_free_varset_ext].
+    + rewrite abstracts_indices_relabel_absidx.
+      cbn -[abstracts_indices].
+      rewrite abstracts_indices_relabel_abs.
+      intros _ (i & -> & Hi)%elem_of_map.
+      rewrite lookup_union.
+      rewrite (lookup_kmap_None (bcons false) _ _).2 by lia.
+      now rewrite (left_id None _).
+    + rewrite ntl_free_varset_relabel_absidx, ntl_free_varset_relabel_ntl_free.
+      intros _ (i & -> & Hi)%elem_of_map.
+      rewrite (lookup_kmap _).
+      unfold make_vecs_map.
+      rewrite 4 vzip_map_l, 4 vec_to_list_map.
+      rewrite <- 4 (kmap_list_to_map _).
+      rewrite 2 lookup_union.
+      destruct i as [i|i|].
+      * replace (i~1) with ((bcons true ∘ Pos.of_succ_nat) i) by now cbn; lia.
+        rewrite (lookup_kmap_None (bcons false ∘ _) _ _).2 by now cbn; lia.
+        rewrite (lookup_kmap _).
+        cbn.
+        replace (_~1) with ((bcons true ∘ Pos.of_succ_nat) (m + i)) by now cbn; lia.
+        (* change (?x~1) with ((bcons true ∘ Pos.of_succ_nat) i). *)
+        rewrite (lookup_kmap _).
+        rewrite (lookup_kmap_None _ _ _).2 by now cbn; lia.
+        f_equal.
+        rewrite vec_to_list_zip_with, vec_to_list_seq.
+        rewrite <- (length_vec_to_list wr) at 1.
+        rewrite <- imap_to_zip_with_seq.
+        rewrite vec_to_list_zip_with, vec_to_list_seq.
+        rewrite <- (length_vec_to_list (wl +++ wr)) at 1.
+        rewrite <- imap_to_zip_with_seq.
+        rewrite (lookup_list_to_map_imap id id _ (pos_to_nat_pred i)).
+        rewrite (lookup_list_to_map_imap id id _ (m + i)).
+        rewrite 2 option_fmap_id.
+        rewrite vec_to_list_app.
+        symmetry.
+        rewrite lookup_app_r; [f_equal; rewrite length_vec_to_list; lia|].
+        rewrite length_vec_to_list.
+        lia.
+      * replace (i~0) with ((bcons false ∘ Pos.of_succ_nat) i) by now cbn; lia.
+        rewrite (lookup_kmap_None (bcons true ∘ _) _ _).2 by now cbn; lia.
+        rewrite (lookup_kmap _).
+        cbn.
+        replace (_~0) with ((bcons false ∘ Pos.of_succ_nat) (i)) by now cbn; lia.
+        rewrite (lookup_kmap _).
+        rewrite (lookup_kmap_None _ _ _).2 by now cbn; lia.
+        f_equal.
+        rewrite vec_to_list_zip_with, vec_to_list_seq.
+        rewrite <- (length_vec_to_list vl) at 1.
+        rewrite <- imap_to_zip_with_seq.
+        rewrite vec_to_list_zip_with, vec_to_list_seq.
+        rewrite <- (length_vec_to_list (vl +++ vr)) at 1.
+        rewrite <- imap_to_zip_with_seq.
+        rewrite 2 (lookup_list_to_map_imap id id _ (pos_to_nat_pred i)).
+        rewrite 2 option_fmap_id.
+        rewrite vec_to_list_app.
+        symmetry.
+        apply lookup_app_l.
+        rewrite ntl_free_varset_graph in Hi.
+        rewrite elem_of_list_to_set in Hi.
+        rewrite 2 vec_to_list_map, 2 vec_to_list_seq in Hi.
+        set_unfold in Hi.
+        setoid_rewrite elem_of_seq in Hi.
+        cbn in Hi.
+        rewrite length_vec_to_list.
+        firstorder lia.
+      * rewrite 4(lookup_kmap_None _ _ _).2 by now cbn; lia.
+        done.
+Qed.
+
+Lemma graph_semantics_compose_graphs_alt {n m o}
+  (cohg : TensorGraph n m) (cohg' : TensorGraph m o) :
+  graph_semantics (SR:=SR) (compose_graphs_alt cohg cohg') ≡
+  compose_tensor (graph_semantics cohg) (graph_semantics cohg').
+Proof.
+  unfold compose_graphs_alt.
+  rewrite graph_semantics_add_top_loops.
+  erewrite join_stack_tl_tr_mor by now apply graph_semantics_swapped_stack_graphs.
+  symmetry; apply compose_to_swapped_stack.
 Qed.
 
 (* #[export] Instance CospanHyperGraph_disj {n m} : Disjoint (CospanHyperGraph T n m) :=
